work on FE310 mmio specs

bedrock2/src/Examples/FE310CompilerDemo.v
@@ -14,8 +14,17 @@ Local Instance syntax_parameters : Syntax.parameters := {|
 |}.
 
 From coqutil.Map Require SortedListWord Z_keyed_SortedListMap Empty_set_keyed_map.
-From coqutil Require Word.Interface Word.Naive.
+From coqutil Require Import Word.Interface Word.Naive Z.HexNotation String.
 Require Import bedrock2.Semantics.
+Import List.ListNotations.
+
+Definition patience : Z.                                     exact (10^150). Qed.
+
+Definition otp_base   := Ox"0x00020000". Definition otp_pastend   := Ox"0x00022000".
+Definition hfrosccfg  := Ox"10008000".
+Definition gpio0_base := Ox"0x10012000". Definition gpio0_pastend := Ox"0x10013000".
+Definition uart0_base := Ox"0x10013000". Definition uart0_pastend := Ox"0x10014000".
+Definition uart0_rxdata := Ox"10013004". Definition uart0_txdata := Ox"10013000".
 
 Local Instance parameters : parameters :=
   let word := Word.Naive.word 32 eq_refl in
@@ -26,5 +35,27 @@ Local Instance parameters : parameters :=
   locals := Z_keyed_SortedListMap.Zkeyed_map _;
   funname_env := Empty_set_keyed_map.map;
   funname_eqb := fun _ _ => true;
-  ext_spec t m a args post := False; (* TODO *)
+  ext_spec t m action args post :=
+    match action, List.map word.unsigned args with
+    | MMOutput, [addr; value] =>
+      if addr =? hfrosccfg                                then Z.testbit value 30 = true else
+      if (gpio0_base <=? addr) && (addr+3 <? gpio0_pastend) then True else
+      if (uart0_base <=? addr) && (addr+3 <? uart0_pastend) then True else
+      False
+      /\ post m []
+    | MMInput, [addr] =>
+      if addr =? hfrosccfg                                  then True else
+      if (  otp_base <=? addr) && (addr+3 <?   otp_pastend) then True else
+      if (gpio0_base <=? addr) && (addr+3 <? gpio0_pastend) then True else
+      if (uart0_base <=? addr) && (addr+3 <? uart0_pastend) then True else
+      False
+      /\ forall v,
+          (patience < Z.of_nat (List.length t) -> addr = uart0_rxdata ->
+            word.and v (word.of_Z 255) = word.of_Z 46) /\
+          (patience < Z.of_nat (List.length t) -> addr = uart0_txdata ->
+            word.and v (word.slu (word.of_Z 1) (word.of_Z 31)) = (word.slu (word.of_Z 1) (word.of_Z 31))) /\
+          post m [v]
+    | _, _ =>
+      False
+    end%list%bool;
 |}.
